try to prove ceval equivalence but failed again (considering change to call in abeval'), update reentry rule with exists, prove the bridge from weak soundness to strong soundness (with weak soundness to be proven)

HoareFunc.v
@@ -15,7 +15,17 @@ exists n, sg n
 
 ceval' sigma <-> ceval *)
 
-Inductive ceval' (sigma : func_context -> public_funcs -> com -> state -> state -> Prop) (fc : func_context) (lf : public_funcs) : com -> state -> state -> Prop :=
+(* Inductive arbitrary_eval' (sigma: func_context -> public_funcs -> com -> state -> state -> Prop) (fc: func_context) (lf: public_funcs): unit_state -> unit_state -> unit_state -> Prop :=
+  | ArE'_nil: forall loc gl, arbitrary_eval' sigma fc lf loc gl gl
+  | ArE'_cons: forall loc loc1 loc2 gl1 gl2 gl3 f,
+      In f lf ->
+      sigma fc lf (func_bdy f) (loc1, gl1) (loc2, gl2) ->
+      arbitrary_eval' sigma fc lf loc gl2 gl3 ->
+      arbitrary_eval' sigma fc lf loc gl1 gl3. *)
+
+Definition semantic : Type := func_context -> public_funcs -> com -> state -> state -> Prop.
+
+Inductive ceval' (sigma : semantic) (fc : func_context) (lf : public_funcs) : com -> state -> state -> Prop :=
   | E'_Skip : forall st,
       ceval' sigma fc lf CSkip st st
   | E'_Ass : forall st X a n,
@@ -47,15 +57,17 @@ Inductive ceval' (sigma : func_context -> public_funcs -> com -> state -> state 
   | E'_Reentry : forall loc glb1 glb2,
       arbitrary_eval' sigma fc lf loc glb1 glb2 ->
       ceval' sigma fc lf CReentry (loc, glb1) (loc, glb2)
-with arbitrary_eval' (sigma: func_context -> public_funcs -> com -> state -> state -> Prop) (fc: func_context) (lf: public_funcs): unit_state -> unit_state -> unit_state -> Prop :=
+with arbitrary_eval' (sigma: semantic) (fc: func_context) (lf: public_funcs): unit_state -> unit_state -> unit_state -> Prop :=
   | ArE'_nil: forall loc gl, arbitrary_eval' sigma fc lf loc gl gl
   | ArE'_cons: forall loc loc1 loc2 gl1 gl2 gl3 f,
-                In f lf ->
-                sigma fc lf (func_bdy f) (loc1, gl1) (loc2, gl2) ->
-                arbitrary_eval' sigma fc lf loc gl2 gl3 ->
-                arbitrary_eval' sigma fc lf loc gl1 gl3.
+      In f lf ->
+      sigma fc lf (func_bdy f) (loc1, gl1) (loc2, gl2) ->
+      arbitrary_eval' sigma fc lf loc gl2 gl3 ->
+      arbitrary_eval' sigma fc lf loc gl1 gl3.
 
-Fixpoint sg (n : nat) : func_context -> public_funcs -> com -> state -> state -> Prop :=
+Module FixpointSigma.
+
+Fixpoint sg (n : nat) : semantic :=
   match n with
   | 0 => fun _ _ _ _ _ => False
   | S n => ceval' (sg n)
@@ -228,7 +240,7 @@ Proof.
   }
 Qed.
 
-Lemma sg_n_ceval_equiv n fc lf: forall c st1 st2,
+Lemma sg_n_ceval n fc lf: forall c st1 st2,
   sg n fc lf c st1 st2 -> ceval fc lf c st1 st2.
 Proof.
   induction n; intros.
@@ -255,7 +267,7 @@ Proof.
         ++ apply IHarbitrary_eval'.
 Qed.
 
-Lemma ceval_sg_n_equiv fc lf: forall c st1 st2,
+Lemma ceval_sg_n fc lf: forall c st1 st2,
   ceval fc lf c st1 st2 ->
   exists n, sg n fc lf c st1 st2.
 Proof.
@@ -286,13 +298,8 @@ Ltac pass := pose proof pass' as Htest; inversion Htest.
 
 (* One way does not work *)
 Lemma ceval'_ceval (fc: func_context) (lf: public_funcs) (c: com) (st1 st2: state) :
-  ceval' sigma fc lf c st1 st2 -> ceval fc lf c st1 st2
-with abeval'_abeval (fc: func_context) (lf: public_funcs) (loc glb1 glb2: unit_state) :
-  arbitrary_eval' sigma fc lf loc glb1 glb2 -> arbitrary_eval fc lf loc glb1 glb2.
+  ceval' sigma fc lf c st1 st2 -> ceval fc lf c st1 st2.
 Proof.
-(* This branch is save now. *)
-{
-  clear ceval'_ceval.
   intros.
   induction H.
   - apply E_Skip.
@@ -304,21 +311,22 @@ Proof.
   - apply E_WhileTrue with st2; auto.
   - destruct H as [n ?].
     eapply E_Call.
-    apply sg_n_ceval_equiv in H.
+    apply sg_n_ceval in H.
     apply H.
   - apply E_Reentry.
     induction H.
     + apply ArE_nil.
     + destruct H0.
-      apply sg_n_ceval_equiv in H0.
+      apply sg_n_ceval in H0.
       eapply ArE_cons.
       apply H.
       apply H0.
       apply IHarbitrary_eval'.
-}
-(* This branch has trouble. *)
-{
-  clear abeval'_abeval.
+Qed.
+
+Lemma abeval'_abeval (fc: func_context) (lf: public_funcs) (loc glb1 glb2: unit_state) :
+  arbitrary_eval' sigma fc lf loc glb1 glb2 -> arbitrary_eval fc lf loc glb1 glb2.
+Proof.
   intros.
   induction H.
   + apply ArE_nil.
@@ -327,6 +335,33 @@ Proof.
     apply ceval'_ceval in H0.
     pose proof ArE_cons _ _ _ _ _ _ _ _ _ H H0 IHarbitrary_eval'.
     apply H2.
+Qed.
+
+Lemma ceval_ceval' (fc: func_context) (lf: public_funcs) (c: com) (st1 st2: state) :
+  ceval fc lf c st1 st2 -> ceval' sigma fc lf c st1 st2
+with abeval_abeval' (fc: func_context) (lf: public_funcs) (loc glb1 glb2: unit_state) :
+  arbitrary_eval fc lf loc glb1 glb2 -> arbitrary_eval' sigma fc lf loc glb1 glb2.
+Proof.
+{
+  clear ceval_ceval'.
+  intros.
+  induction H.
+  - apply E'_Skip.
+  - apply E'_Ass; auto.
+  - apply E'_Seq with st2; auto.
+  - apply E'_IfTrue; auto.
+  - apply E'_IfFalse; auto.
+  - apply E'_WhileFalse; auto.
+  - apply E'_WhileTrue with st2; auto.
+  - eapply E'_Call.
+    rewrite sigma_ceval'_equiv.
+    apply IHceval.
+  - apply E'_Reentry.
+    apply abeval_abeval'.
+    exact H.
+}
+{
+  pass.
 }
 Admitted.
 
@@ -335,80 +370,17 @@ Lemma ceval'_ceval_equiv (fc: func_context) (lf: public_funcs) (c: com) (st1 st2
 with abeval'_abeval_equiv (fc: func_context) (lf: public_funcs) (loc glb1 glb2: unit_state) :
   arbitrary_eval' sigma fc lf loc glb1 glb2 <-> arbitrary_eval fc lf loc glb1 glb2.
 Proof.
-  {
-    clear ceval'_ceval_equiv.
-    split; intros.
-    {
-      induction H.
-      - apply E_Skip.
-      - apply E_Ass; auto.
-      - apply E_Seq with st2; auto.
-      - apply E_IfTrue; auto.
-      - apply E_IfFalse; auto.
-      - apply E_WhileFalse; auto.
-      - apply E_WhileTrue with st2; auto.
-      - destruct H as [n ?].
-        eapply E_Call.
-        apply sg_n_ceval_equiv in H.
-        apply H.
-      - apply E_Reentry.
-        induction H.
-        + apply ArE_nil.
-        + destruct H0.
-          apply sg_n_ceval_equiv in H0.
-          eapply ArE_cons.
-          apply H.
-          apply H0.
-          apply IHarbitrary_eval'.
-(*         pass. *)
-        (* apply E_Reentry.
-        apply abeval'_abeval_equiv.
-        apply H. *)
-    }
-    {
-      induction H.
-      - apply E'_Skip.
-      - apply E'_Ass; auto.
-      - apply E'_Seq with st2; auto.
-      - apply E'_IfTrue; auto.
-      - apply E'_IfFalse; auto.
-      - apply E'_WhileFalse; auto.
-      - apply E'_WhileTrue with st2; auto.
-      - pass.
-        (* eapply E'_Call.
-        rewrite sigma_ceval'_equiv.
-        apply IHceval. *)
-      - pass.
-        (* apply E'_Reentry.
-        rewrite abeval'_abeval_equiv.
-        auto. *)
-    }
-  }
-  {
-    clear abeval'_abeval_equiv.
-    split; intros.
-    {
-      induction H.
-      + apply ArE_nil.
-      + pass.
-        (* apply sigma_ceval'_equiv in H0.
-        apply ceval'_ceval_equiv in H0.
-        pose proof ArE_cons _ _ _ _ _ _ _ _ _ H H0 IHarbitrary_eval'.
-        apply H2. *)
-    }
-    {
-      induction H.
-      + apply ArE'_nil.
-      + pass.
-        (* rewrite <- ceval'_ceval_equiv, <- sigma_ceval'_equiv in H0.
-        eapply ArE'_cons.
-        * apply H.
-        * apply H0.
-        * apply IHarbitrary_eval. *)
-    }
-  }
+  - clear ceval'_ceval_equiv.
+    pose proof ceval_ceval' fc lf c st1 st2.
+    pose proof ceval'_ceval fc lf c st1 st2.
+    tauto.
+  - clear abeval'_abeval_equiv.
+    pose proof abeval_abeval' fc lf loc glb1 glb2.
+    pose proof abeval'_abeval fc lf loc glb1 glb2.
+    tauto.
 Qed.
 
+End FixpointSigma.
 
 Definition func_predicate : Type := func -> Assertion -> Assertion -> Prop.
 
@@ -423,11 +395,11 @@ Notation "{{ P }}  c  {{ Q }}" :=
 
 Inductive provable (fc : func_context) (lf : public_funcs) (fp : func_predicate) : hoare_triple -> Prop :=
   (* fixed reentry *)
-  | hoare_reentry : forall P I,
-      localp P ->
-      globalp I ->
-      (forall f, In f lf -> fp f I I) ->
-      provable fc lf fp ({{P AND I}} CReentry {{P AND I}})
+  | hoare_reentry : forall A (P I: A -> Assertion),
+    (forall x, localp (P x)) ->
+    (forall x,  globalp (I x))->
+      (forall f x, In f lf -> fp f (I x) (I x)) ->
+      provable fc lf fp ({{fun st => exists x, P x st /\ I x st}} CReentry {{fun st => exists x, P x st /\ I x st}})
   (* function predicate call *)
   | hoare_call : forall f pv P Q R,
       globalp Q ->
@@ -447,7 +419,7 @@ Inductive provable (fc : func_context) (lf : public_funcs) (fp : func_predicate)
       provable fc lf fp ({{ P AND {[b]} }} c1 {{ Q }}) ->
       provable fc lf fp ({{ P AND NOT {[b]} }} c2 {{ Q }}) ->
       provable fc lf fp ({{ P }} If b Then c1 Else c2 EndIf {{ Q }})
-  | hoare_while_linear : forall P (b : bexp) c,
+  | hoare_while : forall P (b : bexp) c,
     provable fc lf fp ({{P AND {[b]}}} c {{P}}) ->
     provable fc lf fp ({{P}} While b Do c EndWhile {{P AND NOT {[b]}}})
   | hoare_consequence : forall (P P' Q Q' : Assertion) c,
@@ -457,45 +429,140 @@ Inductive provable (fc : func_context) (lf : public_funcs) (fp : func_predicate)
       provable fc lf fp ({{P}} c {{Q}}).
 Notation "fc lf fp |--  tr" := (provable fc lf fp tr) (at level 91, no associativity).
 
-Definition triple_valid (fc : func_context) (lf : public_funcs) (tr : hoare_triple) : Prop :=
+Definition triple_valid (sigma: semantic) (fc : func_context) (lf : public_funcs) (tr : hoare_triple) : Prop :=
   match tr with
   | {{P}} c {{Q}} =>
-    forall st1 st2, P st1 -> ceval fc lf c st1 st2 -> Q st2
+    forall st1 st2, P st1 -> sigma fc lf c st1 st2 -> Q st2
   end.
-Notation "fc lf |== tr" := (triple_valid fc lf tr) (at level 91, no associativity).
+Notation "sigma fc lf |== tr" := (triple_valid sigma fc lf tr) (at level 91, no associativity).
 
-Definition fp_valid (fc : func_context) (lf : public_funcs) (fp : func_predicate) : Prop :=
-  forall f P Q st1 st2,
-    fp f P Q -> P st1 -> sigma fc lf (func_bdy f) st1 st2 -> Q st2.
-Notation "fc lf ||== fp" := (fp_valid fc lf fp) (at level 91, no associativity).
+Definition valid (fc: func_context) (lf: public_funcs) (tr: hoare_triple) : Prop := triple_valid ceval fc lf tr.
+Notation "fc lf |== tr" := (valid fc lf tr) (at level 91, no associativity).
 
-Definition weak_valid (fc : func_context) (lf : public_funcs) (fp : func_predicate) (tr : hoare_triple) : Prop :=
-  fp_valid fc lf fp ->
-  triple_valid fc lf tr.
-Notation "fc lf fp |== tr" := (weak_valid fc lf fp tr) (at level 91, no associativity).
+Definition fp_valid (sigma: semantic) (fc : func_context) (lf : public_funcs) (fp : func_predicate) : Prop :=
+  forall f P Q,
+(*     fp f P Q -> P st1 -> ceval fc lf (func_bdy f) st1 st2 -> Q st2. *)
+    fp f P Q -> triple_valid sigma fc lf ({{P}} (func_bdy f) {{Q}}).
+Notation "sigma fc lf ||== fp" := (fp_valid sigma fc lf fp) (at level 91, no associativity).
+(* delta f P Q -> delta |== P f Q *)
 
-Theorem hoare_sound_weak : forall fc lf fp tr,
+(*
+  sg n |= delta -> P st1 -> ceval' (sg n) c st1 st2 -> Q st2
+*)
+
+(** Weak Valid *)
+Definition weak_valid (sigma: semantic) (fc : func_context) (lf : public_funcs) (fp : func_predicate) (tr : hoare_triple) : Prop :=
+  fp_valid sigma fc lf fp ->
+  triple_valid (ceval' sigma) fc lf tr.
+Notation "sigma fc lf fp |== tr" := (weak_valid sigma fc lf fp tr) (at level 91, no associativity).
+
+Lemma reentry_sound_weak sigma fc lf (fp: func_predicate) :
+  forall A (P I: A -> Assertion),
+  (forall x, localp (P x)) ->
+  (forall x, globalp (I x)) ->
+  (forall f x, In f lf -> fp f (I x) (I x)) ->
+  weak_valid sigma fc lf fp ({{fun st => exists x, P x st /\ I x st}} CReentry {{fun st => exists x, P x st /\ I x st}}).
+Proof.
+  unfold weak_valid, fp_valid, triple_valid.
+  unfold andp.
+  intros A P I Hloc Hglb.
+  intros.
+  destruct H1 as [? [? ?]].
+  exists x.
+  inversion H2; subst.
+  split; [eapply Hloc; apply H1 |].
+  clear H1 H2.
+  induction H4; [exact H3 |].
+  apply IHarbitrary_eval'; clear IHarbitrary_eval'.
+  pose proof H0 _ _ _ (H _ _ H1) _ (loc2, gl2) (Hglb _ _ loc1 _ H3) H2.
+  eapply Hglb.
+  apply H5.
+Qed.
+
+Theorem hoare_sound_weak : forall sigma fc lf fp tr,
   provable fc lf fp tr ->
-  weak_valid fc lf fp tr.
+  weak_valid sigma fc lf fp tr.
 Proof.
   intros.
-  induction H; unfold weak_valid, fp_valid, triple_valid; intros.
+  induction H.
+  - apply reentry_sound_weak; auto.
+  - admit.
 Admitted.
+(** [] *)
+
+(** Soundness *)
+Import FixpointSigma.
+
+Lemma sg_n_fp_valid : forall n fc lf (fp: func_predicate),
+  (forall f P Q, fp f P Q ->
+    provable fc lf fp ({{P}} (func_bdy f) {{Q}})) ->
+  fp_valid (sg n) fc lf fp.
+Proof.
+  intros.
+  induction n; intros.
+  - unfold fp_valid, triple_valid.
+    simpl.
+    intros.
+    inversion H2.
+  - unfold fp_valid, triple_valid.
+    intros.
+    pose proof H f P Q H0.
+    apply (hoare_sound_weak (sg n)) in H3.
+    unfold weak_valid in H3.
+    specialize (H3 IHn).
+    simpl in H2, H3.
+    eapply H3.
+    + apply H1.
+    + apply H2.
+Qed.
+
+Lemma sigma_fp_valid : forall fc lf (fp: func_predicate),
+  (forall f P Q, fp f P Q ->
+    provable fc lf fp ({{P}} (func_bdy f) {{Q}})) ->
+  fp_valid sigma fc lf fp.
+Proof.
+  intros.
+  unfold fp_valid, triple_valid.
+  intros.
+  destruct H2 as [n ?].
+  pose proof sg_n_fp_valid n fc lf fp H.
+  unfold fp_valid, triple_valid in H3.
+  eapply H3.
+  - apply H0.
+  - apply H1.
+  - apply H2.
+Qed.
 
 (* (Delta P f Q -> Delta |-- P f Q) -> Delta |-- P c Q -> |== P c Q *)
 Theorem hoare_sound: forall fc lf (fp : func_predicate),
   (forall f P Q, fp f P Q ->
       provable fc lf fp ({{P}} (func_bdy f) {{Q}})) ->
   forall tr, provable fc lf fp tr ->
-      triple_valid fc lf tr.
+      valid fc lf tr.
 Proof.
   intros.
-  pose proof hoare_sound_weak _ _ _ _ H0.
-Admitted.
+  pose proof sigma_fp_valid _ _ _ H.
+  pose proof hoare_sound_weak sigma _ _ _ _ H0 H1.
+  destruct tr.
+  simpl in *.
+  intros.
+  eapply H2.
+  - apply H3.
+  - rewrite ceval'_ceval_equiv.
+    apply H4.
+Qed.
+(** [] *)
+
+(** Completeness *)
+Definition reentry_semantic fc lf (st1 st2 : state) : Prop :=
+  match st1, st2 with
+  | (loc1, glb1), (loc2, glb2) =>
+      arbitrary_eval fc lf loc1 glb1 glb2 /\ loc1 = loc2
+  end.
 
 Theorem hoare_complete: forall fc lf tr,
   triple_valid fc lf tr ->
-  exists fp, provable fc lf fp tr.
+  exists fp, provable fc lf fp tr. (* /\ fp |- forall tr in fp *)
 Proof.
   intros.
   destruct tr.
@@ -506,12 +573,25 @@ Proof.
   - admit.
   - admit.
   - admit.
-  - (* how to construct fp *)
-    exists (fun f I I => provable).
+  - (* TODO: global I? split into two *)
+(*     remember ((fun st => exists st0, P st0 /\ reentry_semantic fc lf st0 st):Assertion) as I. *)
+    (* assert (globalp I).
+    {
+      unfold globalp.
+      intros.
+      subst.
+      destruct H0 as [st0 [? ?]].
+      destruct st0 as [loc0 glb0].
+      admit.
+    } *)
+    (* TODO: how to construct fp *)
+    Print func_predicate.
+    remember (fun (f: func) P Q => In f lf -> P = I /\ Q = I) as fp.
+    exists fp.
+    eapply hoare_consequence.
     
-    
-    remember ((fun st => exists st0, P st0 /\ reentry_semantic fc lf st0 st):Assertion) as I.
 Admitted.
+(** [] *)
 
 (*
 Definition fp_valid (fc : func_context) (lf : public_funcs) (fp : func_predicate) : Prop :=
